backend/LTL.v
@@ -152,7 +152,7 @@ Inductive state : Type :=
       forall (stack: list stackframe) (**r call stack *)
              (f: fundef)              (**r function to call *)
              (ls: locset)             (**r location state of caller *)
-             (m: mem),                (**r memory state *)
+             (m: mem)(sz:Z),                (**r memory state *)
       state
   | Returnstate:
       forall (stack: list stackframe) (**r call stack *)
@@ -160,7 +160,9 @@ Inductive state : Type :=
              (m: mem),                (**r memory state *)
       state.
 
+Section ORACLE.
 
+Variable fn_stack_requirements : ident -> Z.
 Section RELSEM.
 
 Variable ge: genv.
@@ -199,6 +201,12 @@ Definition parent_locset (stack: list stackframe) : locset :=
   | Stackframe f sp ls bb :: stack' => ls
   end.
 
+Definition ros_is_function (ros: mreg + ident) (rs: locset) (i: ident) : Prop :=
+  match ros with
+  | inl r => exists b o, rs (R r) = Vptr b o /\ Genv.find_symbol ge i = Some b
+  | inr symb => i = symb
+  end.
+
 Inductive step: state -> trace -> state -> Prop :=
   | exec_start_block: forall s f sp pc rs m bb,
       (fn_code f)!pc = Some bb ->
@@ -229,24 +237,29 @@ Inductive step: state -> trace -> state -> Prop :=
       rs' = undef_regs (destroyed_by_store chunk addr) rs ->
       step (Block s f sp (Lstore chunk addr args src :: bb) rs m)
         E0 (Block s f sp bb rs' m')
-  | exec_Lcall: forall s f sp sig ros bb rs m fd,
+  | exec_Lcall: forall s f sp sig ros bb rs m fd id,
+      ros_is_function ros rs id ->
       find_function ros rs = Some fd ->
       funsig fd = sig ->
       step (Block s f sp (Lcall sig ros :: bb) rs m)
-        E0 (Callstate (Stackframe f sp rs bb :: s) fd rs m)
-  | exec_Ltailcall: forall s f sp sig ros bb rs m fd rs' m',
+        E0 (Callstate (Stackframe f sp rs bb :: s) fd rs
+                      (Mem.push_stage m)
+                      (fn_stack_requirements id))
+  | exec_Ltailcall: forall s f sp sig ros bb rs m fd rs' m' id,
+      ros_is_function ros rs id ->
       rs' = return_regs (parent_locset s) rs ->
       find_function ros rs' = Some fd ->
       funsig fd = sig ->
       Mem.free m sp 0 f.(fn_stacksize) = Some m' ->
       step (Block s f (Vptr sp Ptrofs.zero) (Ltailcall sig ros :: bb) rs m)
-        E0 (Callstate s fd rs' m')
-  | exec_Lbuiltin: forall s f sp ef args res bb rs m vargs t vres rs' m',
+        E0 (Callstate s fd rs' m' (fn_stack_requirements id))
+  | exec_Lbuiltin: forall s f sp ef args res bb rs m vargs t vres rs' m' m'',
       eval_builtin_args ge rs sp m args vargs ->
-      external_call ef ge vargs m t vres m' ->
+      external_call ef ge vargs (Mem.push_stage m) t vres m' ->
+      Mem.pop_stage m' = Some m'' ->
       rs' = Locmap.setres res vres (undef_regs (destroyed_by_builtin ef) rs) ->
       step (Block s f sp (Lbuiltin ef args res :: bb) rs m)
-         t (Block s f sp bb rs' m')
+         t (Block s f sp bb rs' m'')
   | exec_Lbranch: forall s f sp pc bb rs m,
       step (Block s f sp (Lbranch pc :: bb) rs m)
         E0 (State s f sp pc rs m)
@@ -266,20 +279,22 @@ Inductive step: state -> trace -> state -> Prop :=
       Mem.free m sp 0 f.(fn_stacksize) = Some m' ->
       step (Block s f (Vptr sp Ptrofs.zero) (Lreturn :: bb) rs m)
         E0 (Returnstate s (return_regs (parent_locset s) rs) m')
-  | exec_function_internal: forall s f rs m m' sp rs',
+  | exec_function_internal: forall s f rs m m' m'' sp rs' sz,
       Mem.alloc m 0 f.(fn_stacksize) = (m', sp) ->
+      Mem.record_frame_mach m' (Mem.mk_frame sz) = Some m'' ->
       rs' = undef_regs destroyed_at_function_entry (call_regs rs) ->
-      step (Callstate s (Internal f) rs m)
-        E0 (State s f (Vptr sp Ptrofs.zero) f.(fn_entrypoint) rs' m')
-  | exec_function_external: forall s ef t args res rs m rs' m',
+      step (Callstate s (Internal f) rs m sz)
+        E0 (State s f (Vptr sp Ptrofs.zero) f.(fn_entrypoint) rs' m'')
+  | exec_function_external: forall s ef t args res rs m rs' m' sz,
       args = map (fun p => Locmap.getpair p rs) (loc_arguments (ef_sig ef)) ->
       external_call ef ge args m t res m' ->
       rs' = Locmap.setpair (loc_result (ef_sig ef)) res (undef_caller_save_regs rs) ->
-      step (Callstate s (External ef) rs m)
+      step (Callstate s (External ef) rs m sz)
          t (Returnstate s rs' m')
-  | exec_return: forall f sp rs1 bb s rs m,
+  | exec_return: forall f sp rs1 bb s rs m m',
+      Mem.pop_stage m = Some m' ->
       step (Returnstate (Stackframe f sp rs1 bb :: s) rs m)
-        E0 (Block s f sp bb rs m).
+        E0 (Block s f sp bb rs m').
 
 End RELSEM.
 
@@ -295,7 +310,8 @@ Inductive initial_state (p: program): state -> Prop :=
       Genv.find_symbol ge p.(prog_main) = Some b ->
       Genv.find_funct_ptr ge b = Some f ->
       funsig f = signature_main ->
-      initial_state p (Callstate nil f (Locmap.init Vundef) m0).
+      initial_state p (Callstate nil f (Locmap.init Vundef) (Mem.push_stage m0)
+                       (fn_stack_requirements (prog_main p))).
 
 Inductive final_state: state -> int -> Prop :=
   | final_state_intro: forall rs m retcode,
@@ -305,6 +321,7 @@ Inductive final_state: state -> int -> Prop :=
 Definition semantics (p: program) :=
   Semantics step (initial_state p) final_state (Genv.globalenv p).
 
+End ORACLE.
 (** * Operations over LTL *)
 
 (** Computation of the possible successors of a block.
