backend/RTLmachproof.v
@@ -12,6 +12,175 @@
 
 (** Postorder renumbering of RTL control-flow graphs. *)
 
-Require Import Coqlib.
-Require Import RTL.
-Require Import RTLMach.
+Require Import Coqlib Maps.
+Require Import AST Linking.
+Require Import Values Memory Globalenvs Events Smallstep.
+Require Import Op Registers RTL RTLmach.
+(*
+Definition transf_instr (pc:node)(i: RTL.instruction) : instruction :=
+  match i with
+  | RTL.Inop s => Inop s
+  | RTL.Iop op args res s => Iop op args res s
+  | RTL.Iload chunk addr args res s => Iload chunk addr args res s
+  | RTL.Istore chunk addr args src s => Istore chunk addr args src s
+  | RTL.Icall sg ros args res s => Icall sg ros args res s
+  | RTL.Itailcall sg ros args => Itailcall sg ros args
+  | RTL.Ibuiltin ef args res s => Ibuiltin ef args res s
+  | RTL.Icond cond args s1 s2 => Icond cond args s1 s2
+  | RTL.Ijumptable arg tbl => Ijumptable arg tbl
+  | RTL.Ireturn or => Ireturn or
+  end.
+
+Definition transf_function (f: function) : function :=
+  mkfunction
+    f.(RTL.fn_sig)
+    f.(RTL.fn_params)
+    f.(RTL.fn_stacksize)
+    (PTree.map transf_instr f.(RTL.fn_code))
+    f.(RTL.fn_entrypoint).
+
+Definition transf_fundef (fd: RTL.fundef) : fundef :=
+  AST.transf_fundef transf_function fd.
+*)
+Definition transf_program (p: program) : program := p.
+
+
+Definition match_prog (p :RTL.program) (tp:program):= p = tp.
+
+Lemma transf_program_match:
+  forall p, match_prog p (transf_program p).
+Proof.
+  intros. reflexivity.
+Qed.
+
+Section PRESERVATION.
+
+Variables fn_stack_requirements : ident -> Z.
+Variables prog: RTL.program.
+Variables tprog: program.
+Hypothesis TRANSL: match_prog prog tprog.
+Let ge := Genv.globalenv prog.
+Let tge := Genv.globalenv tprog.
+
+Lemma prog_eq : prog = tprog.
+Proof. auto. Qed.
+
+Lemma genv_eq : ge = tge.
+Proof.
+  unfold match_prog in TRANSL. unfold ge.
+  unfold tge. congruence.
+Qed.
+(*
+Lemma functions_translated:
+  forall v f,
+  Genv.find_funct ge v = Some f ->
+  Genv.find_funct tge v = Some f.
+Proof. apply (Genv.find_funct_transf TRANSL). Qed.
+
+Lemma function_ptr_translated:
+  forall v f,
+  Genv.find_funct_ptr ge v = Some f ->
+  Genv.find_funct_ptr tge v = Some (transf_fundef f).
+Proof. apply (Genv.find_funct_ptr_transf TRANSL). Qed.
+
+Lemma symbols_preserved:
+  forall id,
+  Genv.find_symbol tge id = Genv.find_symbol ge id.
+Proof. apply (Genv.find_symbol_transf TRANSL). Qed.
+
+Lemma senv_preserved:
+  Senv.equiv ge tge.
+Proof. apply (Genv.senv_transf TRANSL). Qed.
+
+Lemma sig_preserved:
+  forall f, funsig (transf_fundef f) = RTL.funsig f.
+Proof.
+  destruct f; reflexivity.
+Qed.
+
+Lemma find_function_translated:
+  forall ros rs fd,
+  RTL.find_function ge ros rs = Some fd ->
+  find_function tge ros rs = Some (transf_fundef fd).
+Proof.
+  unfold find_function; unfold RTL.find_function; intros. destruct ros as [r|id].
+  eapply functions_translated; eauto.
+  rewrite symbols_preserved. destruct (Genv.find_symbol ge id); try congruence.
+  eapply function_ptr_translated; eauto.
+Qed.
+*)
+Lemma stage_size_head_le_all : forall s : Mem.stage,
+    Mem.size_of_head_frame s <= Mem.size_of_all_frames s.
+Proof.
+  intros. induction s.
+  - simpl. lia.
+  - simpl.  generalize (Mem.size_of_all_frames_pos s).
+    lia.
+Qed.
+Lemma stack_size_mach_le_vm : forall stk : Mem.stackadt,
+    Mem.stack_size_mach stk <= Mem.stack_size_vm stk.
+Proof.
+  intros. induction stk.
+  - simpl. lia.
+  - simpl. generalize (stage_size_head_le_all a).
+    lia.
+Qed.
+
+Definition match_states (s1 s2:state):  Prop := s1 = s2.
+
+Lemma step_simulation:
+  forall S1 t S2, RTL.step fn_stack_requirements ge S1 t S2 ->
+  forall S1', match_states S1 S1' ->
+  exists S2', step fn_stack_requirements tge S1' t S2' /\ match_states S2 S2'.
+Proof.
+  intros. inv H0. rewrite <- genv_eq. exists S2.
+  inv H; split.
+  constructor; auto. reflexivity.
+  econstructor; eauto. reflexivity.
+  eapply exec_Iload; eauto.  reflexivity.
+  eapply exec_Istore; eauto. reflexivity.
+  econstructor; eauto. reflexivity.
+  econstructor; eauto. reflexivity.
+  econstructor; eauto. reflexivity.
+  eapply exec_Icond; eauto. reflexivity.
+  eapply exec_Ijumptable; eauto. reflexivity.
+  eapply exec_Ireturn; eauto. reflexivity.
+  econstructor. apply H0.
+  apply Mem.record_frame_vm_result in H1 as H2.
+  apply Mem.record_frame_vm_size in H1 as H3.
+  unfold Mem.record_frame_mach. rewrite H2.
+  generalize (stack_size_mach_le_vm (Mem.stack (Mem.support m''))).
+  intro.
+  assert (Mem.stack_size_mach (Mem.stack (Mem.support m'')) <= Mem.max_stacksize) by lia.
+  apply zle_true. auto. reflexivity.
+  econstructor; eauto. reflexivity.
+  econstructor; eauto. reflexivity.
+Qed.
+
+Lemma transl_initial_states:
+  forall S, RTL.initial_state fn_stack_requirements prog S ->
+  exists R, initial_state fn_stack_requirements tprog R /\ match_states S R.
+Proof.
+  intros. exists S. split. inv TRANSL.
+  inv H. econstructor; eauto. reflexivity.
+Qed.
+
+Lemma transl_final_states:
+  forall S R r,
+  match_states S R -> RTL.final_state S r -> final_state R r.
+Proof.
+  intros. inv H0. inv H. constructor.
+Qed.
+
+Theorem transf_program_correct:
+  forward_simulation (RTL.semantics fn_stack_requirements prog)
+                     (semantics fn_stack_requirements tprog).
+Proof.
+  eapply forward_simulation_step.
+  inv TRANSL. auto.
+  eexact transl_initial_states.
+  eexact transl_final_states.
+  exact step_simulation.
+Qed.
+
+End PRESERVATION.
