backend/RTLtyping.v
@@ -24,7 +24,7 @@ Require Import Values.
 Require Import Integers.
 Require Import Memory.
 Require Import Events.
-Require Import RTL.
+Require Import RTL RTLmach.
 Require Import Conventions.
 
 (** * The type system *)
@@ -893,11 +893,11 @@ Inductive wt_state: state -> Prop :=
         (WT_RS: wt_regset env rs),
       wt_state (State s f sp pc rs m)
   | wt_state_call:
-      forall s f args m,
+      forall s f args m sz,
       wt_stackframes s (funsig f) ->
       wt_fundef f ->
       Val.has_type_list args (sig_args (funsig f)) ->
-      wt_state (Callstate s f args m)
+      wt_state (Callstate s f args m sz)
   | wt_state_return:
       forall s v m sg,
       wt_stackframes s sg ->
@@ -921,8 +921,10 @@ Hypothesis wt_p: wt_program p.
 
 Let ge := Genv.globalenv p.
 
+Variable fn_stack_requirements : ident -> Z.
+
 Lemma subject_reduction:
-  forall st1 t st2, step ge st1 t st2 ->
+  forall st1 t st2, step fn_stack_requirements ge st1 t st2 ->
   forall (WT: wt_state st1), wt_state st2.
 Proof.
   induction 1; intros; inv WT;
@@ -936,29 +938,31 @@ Proof.
   (* Istore *)
   econstructor; eauto.
   (* Icall *)
+  try (generalize (wt_instrs _ _ WT_FN pc _ H0); intros WTI).
   assert (wt_fundef fd).
-    destruct ros; simpl in H0.
+    destruct ros; simpl in H1.
     pattern fd. apply Genv.find_funct_prop with fundef unit p (rs#r).
-    exact wt_p. exact H0.
-    caseEq (Genv.find_symbol ge i); intros; rewrite H1 in H0.
+    exact wt_p. exact H1.
+    caseEq (Genv.find_symbol ge i); intros; rewrite H2 in H1.
     pattern fd. apply Genv.find_funct_ptr_prop with fundef unit p b.
-    exact wt_p. exact H0.
+    exact wt_p. exact H1.
     discriminate.
   econstructor; eauto.
   econstructor; eauto. inv WTI; auto.
-  inv WTI. rewrite <- H8. apply wt_regset_list. auto.
+  inv WTI. rewrite <- H9. apply wt_regset_list. auto.
   (* Itailcall *)
+  try (generalize (wt_instrs _ _ WT_FN pc _ H0); intros WTI).
   assert (wt_fundef fd).
-    destruct ros; simpl in H0.
+    destruct ros; simpl in H1.
     pattern fd. apply Genv.find_funct_prop with fundef unit p (rs#r).
-    exact wt_p. exact H0.
-    caseEq (Genv.find_symbol ge i); intros; rewrite H1 in H0.
+    exact wt_p. exact H1.
+    caseEq (Genv.find_symbol ge i); intros; rewrite H2 in H1.
     pattern fd. apply Genv.find_funct_ptr_prop with fundef unit p b.
-    exact wt_p. exact H0.
+    exact wt_p. exact H1.
     discriminate.
   econstructor; eauto.
   inv WTI. apply wt_stackframes_change_sig with (fn_sig f); auto.
-  inv WTI. rewrite <- H7. apply wt_regset_list. auto.
+  inv WTI. rewrite <- H8. apply wt_regset_list. auto.
   (* Ibuiltin *)
   econstructor; eauto. eapply wt_exec_Ibuiltin; eauto.
   (* Icond *)
@@ -969,19 +973,19 @@ Proof.
   econstructor; eauto.
   inv WTI; simpl. auto. rewrite <- H3. auto.
   (* internal function *)
-  simpl in *. inv H5.
+  simpl in *. inv H7.
   econstructor; eauto.
-  inv H1. apply wt_init_regs; auto. rewrite wt_params0. auto.
+  inv H2. apply wt_init_regs; auto. rewrite wt_params0. auto.
   (* external function *)
   econstructor; eauto.
   eapply external_call_well_typed; eauto.
   (* return *)
-  inv H1. econstructor; eauto.
-  apply wt_regset_assign; auto. rewrite H10; auto.
+  inv H2. econstructor; eauto.
+  apply wt_regset_assign; auto. rewrite H11; auto.
 Qed.
 
 Lemma wt_initial_state:
-  forall S, initial_state p S -> wt_state S.
+  forall S, initial_state fn_stack_requirements p S -> wt_state S.
 Proof.
   intros. inv H. constructor. constructor. rewrite H3; auto.
   pattern f. apply Genv.find_funct_ptr_prop with fundef unit p b.
