backend/Renumberproof.v
@@ -15,7 +15,7 @@
 Require Import Coqlib Maps Postorder.
 Require Import AST Linking.
 Require Import Values Memory Globalenvs Events Smallstep.
-Require Import Op Registers RTL Renumber.
+Require Import Op Registers RTL RTLmach Renumber.
 
 Definition match_prog (p tp: RTL.program) :=
   match_program (fun ctx f tf => tf = transf_fundef f) eq p tp.
@@ -28,6 +28,7 @@ Qed.
 
 Section PRESERVATION.
 
+Variables fn_stack_requirements : ident -> Z.
 Variables prog tprog: program.
 Hypothesis TRANSL: match_prog prog tprog.
 Let ge := Genv.globalenv prog.
@@ -69,6 +70,19 @@ Proof.
   eapply functions_translated; eauto.
   rewrite symbols_preserved. destruct (Genv.find_symbol ge id); try congruence.
   eapply function_ptr_translated; eauto.
+Qed.
+
+Lemma find_function_id_preserved:
+  forall ros rs id,
+  ros_is_function ge ros rs id ->
+  ros_is_function tge ros rs id.
+Proof.
+  unfold ros_is_function. intros.
+  destruct ros.
+  - destruct H as (b & o & RS & FS).
+  eexists; eexists; split; eauto.
+  rewrite symbols_preserved. auto.
+  - auto.
 Qed.
 
 (** Effect of an injective renaming of nodes on a CFG. *)
@@ -146,19 +160,19 @@ Inductive match_states: RTL.state -> RTL.state -> Prop :=
         (REACH: reach f pc),
       match_states (State stk f sp pc rs m)
                    (State stk' (transf_function f) sp (renum_pc (pnum f) pc) rs m)
-  | match_callstates: forall stk f args m stk'
+  | match_callstates: forall stk f args m stk' sz
         (STACKS: list_forall2 match_frames stk stk'),
-      match_states (Callstate stk f args m)
-                   (Callstate stk' (transf_fundef f) args m)
+      match_states (Callstate stk f args m sz)
+                   (Callstate stk' (transf_fundef f) args m sz)
   | match_returnstates: forall stk v m stk'
         (STACKS: list_forall2 match_frames stk stk'),
       match_states (Returnstate stk v m)
                    (Returnstate stk' v m).
 
 Lemma step_simulation:
-  forall S1 t S2, RTL.step ge S1 t S2 ->
+  forall S1 t S2, step fn_stack_requirements ge S1 t S2 ->
   forall S1', match_states S1 S1' ->
-  exists S2', RTL.step tge S1' t S2' /\ match_states S2 S2'.
+  exists S2', step fn_stack_requirements tge S1' t S2' /\ match_states S2 S2'.
 Proof.
   induction 1; intros S1' MS; inv MS; try TR_AT.
 (* nop *)
@@ -184,12 +198,14 @@ Proof.
 (* call *)
   econstructor; split.
   eapply exec_Icall with (fd := transf_fundef fd); eauto.
+    eapply find_function_id_preserved; eauto.
     eapply find_function_translated; eauto.
     apply sig_preserved.
   constructor. constructor; auto. constructor. eapply reach_succ; eauto. simpl; auto.
 (* tailcall *)
   econstructor; split.
   eapply exec_Itailcall with (fd := transf_fundef fd); eauto.
+    eapply find_function_id_preserved; eauto.
     eapply find_function_translated; eauto.
     apply sig_preserved.
   constructor. auto.
@@ -224,15 +240,15 @@ Proof.
     eapply external_call_symbols_preserved; eauto. apply senv_preserved.
   constructor; auto.
 (* return *)
-  inv STACKS. inv H1.
+  inv STACKS. inv H2.
   econstructor; split.
   eapply exec_return; eauto.
   constructor; auto.
 Qed.
 
 Lemma transf_initial_states:
-  forall S1, RTL.initial_state prog S1 ->
-  exists S2, RTL.initial_state tprog S2 /\ match_states S1 S2.
+  forall S1, initial_state fn_stack_requirements prog S1 ->
+  exists S2, initial_state fn_stack_requirements tprog S2 /\ match_states S1 S2.
 Proof.
   intros. inv H. econstructor; split.
   econstructor.
@@ -240,17 +256,19 @@ Proof.
     rewrite symbols_preserved. rewrite (match_program_main TRANSL). eauto.
     eapply function_ptr_translated; eauto.
     rewrite <- H3; apply sig_preserved.
+  destruct TRANSL as (_&MAIN&_). rewrite MAIN.
   constructor. constructor.
 Qed.
 
 Lemma transf_final_states:
-  forall S1 S2 r, match_states S1 S2 -> RTL.final_state S1 r -> RTL.final_state S2 r.
+  forall S1 S2 r, match_states S1 S2 -> final_state S1 r -> final_state S2 r.
 Proof.
   intros. inv H0. inv H. inv STACKS. constructor.
 Qed.
 
 Theorem transf_program_correct:
-  forward_simulation (RTL.semantics prog) (RTL.semantics tprog).
+  forward_simulation (semantics fn_stack_requirements prog)
+                     (semantics fn_stack_requirements tprog).
 Proof.
   eapply forward_simulation_step.
   apply senv_preserved.
