Makefile
@@ -93,6 +93,7 @@ BACKEND=\
   RTLgen.v RTLgenspec.v RTLgenproof.v \
   Tailcall.v Tailcallproof.v \
   Inlining.v Inliningspec.v Inliningproof.v \
+  RTLmach.v RTLmachproof.v \
   Renumber.v Renumberproof.v \
   RTLtyping.v \
   Kildall.v Liveness.v \
